Move tactics to common file. Add evaluation context lang and STLC extension for it

src/named/IsPfOf.v
@@ -5,7 +5,7 @@ Unset Printing Implicit Defensive.
 Set Bullet Behavior "Strict Subproofs".
 
 From Utils Require Import Utils.
-From Named Require Import Exp ARule Pf PfCore.
+From Named Require Import Exp ARule Pf PfCore PfMatches ParStep.
 Import Exp.Notations Pf.Notations.
 
 Require Import String.
@@ -148,3 +148,207 @@ Inductive is_pf_of_compiler (target : pf_lang)
             (compile target ecmp e2) ->
     is_pf_of_compiler target cmp ((n,p)::ecmp) ((n,term_le_pf c e1 e2 t) :: l).
 Hint Constructors is_pf_of_compiler : pfcore.
+
+
+
+
+(*TODO:move to IsPfOf*)
+Definition get_rule_args_pf := 
+fun r  =>
+match r with
+| sort_rule_pf _ args | term_rule_pf _ args _ => args
+| sort_le_pf c _ _ | term_le_pf c _ _ _ => [seq i.1 | i <- c]
+end.
+Definition get_rule_sort r := 
+match r with
+| sort_rule_pf _ _
+| sort_le_pf _ _ _ => pcon "ERR" [::]
+| term_rule_pf _ _ t
+| term_le_pf _ _ _ t => t
+end.
+
+Lemma elab_sort_by' (l : pf_lang) c : forall n s es,
+    let r := named_list_lookup (sort_rule_pf [::] [::]) l n in
+    let args := get_rule_args_pf r in
+    let c' := get_rule_ctx r in
+    (n, (sort_rule_pf c' args)) \in l ->
+    is_pf_of_wf_args l c s args es c' ->
+    is_pf_of_wf_sort l c (scon n s) (pcon n es).
+Proof.
+  eauto with pfcore.
+Qed.
+
+Lemma elab_term_by' l c : forall n s es t,
+    let r := named_list_lookup (sort_rule_pf [::] [::]) l n in
+    let args := get_rule_args_pf r in
+    let c' := get_rule_ctx r in
+    let t' := get_rule_sort r in
+    (n, (term_rule_pf c' args t')) \in l ->
+    is_pf_of_wf_args l c s args es c' ->
+    t = (pf_subst (with_names_from c' es) t') ->
+    is_pf_of_wf_term l c (con n s) (pcon n es) t.
+Proof.
+  intros; subst;
+  eauto with pfcore.
+Qed.
+
+Ltac break_is_pf_of_wf_args :=
+  cbn;
+  repeat lazymatch goal with
+    | [|- is_pf_of_wf_args _ _ _ (?n::_) _ ((?n,_)::_)] =>
+      eapply elab_args_cons_ex
+    | [|- is_pf_of_wf_args _ _ _ _ _ ((?n,_)::_)] =>
+      eapply elab_args_cons_im
+    | [|- is_pf_of_wf_args _ _ _ _ _ [::]] =>
+      eapply elab_args_nil
+    end.
+
+Ltac solve_sort_equality :=
+  compute;
+  match goal with
+    [|- ?t1 = ?t2] =>
+    reflexivity ||
+    fail "sort" t1 "is not unifiable with sort" t2
+  end.
+  
+Ltac pcon :=
+  lazymatch goal with
+  | [|-is_pf_of_wf_sort ?l ?c ?t ?pt] =>
+    let t' := eval compute in t in
+    let pt' := eval compute in pt in
+    (* should never succeed:
+       assert_fails (is_evar t'; is_evar pt'); *)
+    let c' := eval compute in c in
+    change_no_check (is_pf_of_wf_sort l c' t' pt');
+    eapply elab_sort_by'; [ by compute|break_is_pf_of_wf_args]
+  | [|-is_pf_of_wf_term ?l ?c ?e ?pe ?t] =>
+    let e' := eval compute in e in
+    let pe' := eval compute in pe in
+    (* should never succeed:
+       assert_fails (is_evar e'; is_evar pe'); *)
+    let c' := eval compute in c in
+    let t' := eval compute in t in
+    change_no_check (is_pf_of_wf_term l c' e' pe' t');
+    eapply elab_term_by'; [ by compute| break_is_pf_of_wf_args | solve_sort_equality]
+  end.
+
+(*TODO something funny w/ printed evars in error; 
+  maybe a backtracking thing?
+*)
+Ltac pvar :=
+  eapply elab_term_var;
+      apply named_list_lookup_err_in;
+      match goal with
+        [|- Some ?t = named_list_lookup_err ?c ?x] =>
+        let t' := eval compute in t in
+        let t_r := eval compute in (named_list_lookup_err c x) in
+        change_no_check (Some t' = t_r);
+        compute;
+        reflexivity ||
+        fail "attempted to use var" x "at type" t'
+        "when it has type" t_r
+      end.
+
+(*TODO: move to the right place*)
+Lemma is_pf_of_le_trans l p1 p2 t1 t12 t2
+  : is_pf_of_le l p1 t1 t12 ->
+    is_pf_of_le l p2 t12 t2 ->
+    is_pf_of_le l (trans p1 p2) t1 t2.
+Proof.
+  unfold is_pf_of_le.
+  cbn [proj_l proj_r].
+  easy.
+Qed.
+
+
+Lemma is_pf_of_le_sym l p t1 t2
+  : is_pf_of_le l p t1 t2 ->
+    is_pf_of_le l (sym p) t2 t1.
+Proof.
+  unfold is_pf_of_le.
+  cbn [proj_l proj_r].
+  easy.
+Qed.
+
+
+Lemma is_pf_of_le_refl l t
+  : is_exp t -> is_pf_of_le l t t t.
+Proof.
+Admitted.
+
+  (*rewrite from left to right*)
+    Require Import RuleStep.
+
+    Ltac solve_one_rule_left_to_right_lhs rule_name :=
+    lazymatch goal with
+      [|- is_pf_of_le ?l ?p_evar ?lhs ?rhs] =>
+      tryif is_evar rhs; is_evar p_evar
+      then
+        let x := eval compute in (rule_step_left l rule_name lhs) in
+            lazymatch x with
+            | Some ?p =>
+              let rhs' := eval compute in (proj_r l p) in
+              unify p_evar p;
+              unify rhs' rhs;
+              by compute
+            | None => fail "rule" rule_name
+                           "could not be rewritten from left to right in" lhs
+            end
+      else fail "rhs and p_evar not evars"
+    end.
+
+    (*TODO: reduce code duplication *)
+    Ltac solve_one_rule_right_to_left_rhs rule_name :=
+    lazymatch goal with
+      [|- is_pf_of_le ?l ?p_evar ?lhs ?rhs] =>
+      tryif is_evar lhs; is_evar p_evar
+      then
+        let x := eval compute in (rule_step_right l rule_name rhs) in
+            lazymatch x with
+            | Some ?p =>
+              let lhs' := eval compute in (proj_l l p) in
+              unify p_evar p;
+              unify lhs' lhs;
+              by compute
+            | None => fail "rule" rule_name
+                           "could not be rewritten from right to left in" rhs
+            end
+      else fail "lhs and p_evar not evars"
+      end.
+
+(*TODO: get better errors on these*)
+Ltac le_rewrite rule_name :=
+  first [ eapply is_pf_of_le_trans;
+          [solve_one_rule_left_to_right_lhs rule_name |]
+        | eapply is_pf_of_le_trans;
+          [| eapply is_pf_of_le_sym;
+             solve_one_rule_right_to_left_rhs rule_name]].
+
+Ltac le_rewrite_rtl rule_name :=
+  first [ eapply is_pf_of_le_trans;
+          [eapply is_pf_of_le_sym;
+           solve_one_rule_right_to_left_rhs rule_name |]
+        | eapply is_pf_of_le_trans;
+          [|solve_one_rule_left_to_right_lhs rule_name]].
+
+Ltac le_reflexivity :=
+      apply is_pf_of_le_refl; apply /check_is_expP; by compute.
+
+Ltac reduce fuel :=
+  lazymatch goal with
+    [|- is_pf_of_le ?l ?p_evar ?lhs ?rhs] =>
+    tryif is_evar p_evar
+    then
+      let lhsp := eval compute in (par_step_n l lhs fuel) in
+          let rhsp := eval compute in (par_step_n l rhs fuel) in
+              let lhs' := eval compute in (proj_r l lhsp) in
+                  let rhs' := eval compute in (proj_r l rhsp) in
+                      let p_r := open_constr:(trans _ (sym rhsp)) in
+                      apply (@is_pf_of_le_trans l lhsp p_r lhs lhs' rhs);
+                      [by compute |];
+                      apply (is_pf_of_le_trans (t12 := rhs'));
+                      [| by compute]
+    else fail p_evar "not an evar"
+  end.
+
+Local Open Scope string.
