src/named/SimpleEvalCtx.v
@@ -1,0 +1,157 @@
+
+Require Import mathcomp.ssreflect.all_ssreflect.
+Set Implicit Arguments.
+Unset Strict Implicit.
+Unset Printing Implicit Defensive.
+Set Bullet Behavior "Strict Subproofs".
+
+
+From Ltac2 Require Import Ltac2.
+Set Default Proof Mode "Classic".
+From Utils Require Import Utils.
+From Named Require Import Exp ARule.
+From Named Require Import ImCore Pf PfCore.
+From Named Require Import SimpleVSubst SimpleVSTLC IsPfOf.
+Import Exp.Notations ARule.Notations.
+Require Import String.
+
+Set Default Proof Mode "Classic".
+
+(*An extension to subst_lang *)
+Definition subst_eval_ctx :=
+  [:: (* TODO: do I want a substitution eval ctx? I think no
+         [:> "G1" : #"env", "G2" : #"env", "G3" : #"env", "f" : #"sub" %"G1" %"G2", "g" : #"sub" %"G2" %"G3", "A" : #"ty", "e" : #"el" %"G3" %"A"
+        ----------------------------------------------- ("el_subst_cmp")
+        #"el_subst" %"f" (#"el_subst" %"g" %"e") = #"el_subst" (#"cmp" %"f" %"g") %"e" : #"el" %"G1" %"A"
+    ]%arule;
+  [:> "G" : #"env", "A" : #"ty", "B": #"ty", "E" : #"Ectx" %"G'" %"A" %"B"
+        ----------------------------------------------- ("E_subst_id")
+        #"E_subst" #"id" %"E" = %"E" : #"Ectx" %"G'" %"A" %"B"
+    ]%arule;
+  [:| "G" : #"env", "G'" : #"env", "g" : #"sub" %"G" %"G'",
+      "A" : #"ty", "B" : #"ty", "E" : #"Ectx" %"G" %"A" %"B"
+        -----------------------------------------------
+        #"E_subst" "g" "E" : #"Ectx" %"G'" %"A" %"B"
+    ];*)
+     [:> "G" : #"env", "A" : #"ty",
+         "e" : #"el" %"G" %"A"
+        ----------------------------------------------- ("plug hole")
+        #"plug" #"[ ]" %"e" = %"e" : #"el" %"G" %"A"
+     ];
+     [:| "G" : #"env", "A" : #"ty", "B" : #"ty",
+         "E" : #"Ectx" %"G" %"A" %"B",
+         "e" : #"el" %"G" %"A"
+        -----------------------------------------------
+        #"plug" "E" "e" : #"el" %"G" %"B"
+     ];
+     [:| "G" : #"env", "A" : #"ty"
+        -----------------------------------------------
+        #"[ ]" : #"Ectx" %"G" %"A" %"A"
+     ];
+     [s| "G" : #"env", "A" : #"ty", "B" : #"ty"
+        -----------------------------------------------
+        #"Ectx" "G" "A" "B" srt
+     ]
+  ]%arule.
+
+(*TODO: should be proven in subst file*)
+Lemma is_pf_of_wf_lang_vsubst : is_pf_of_wf_lang subst_lang vsubst_elab.
+Admitted.
+
+Derive subst_eval_ctx_elab
+       SuchThat (is_pf_of_wf_lang (subst_eval_ctx ++ subst_lang) (subst_eval_ctx_elab ++ vsubst_elab)
+         /\ lang_ok (subst_eval_ctx_elab ++ vsubst_elab))
+       As subst_eval_ctx_elab_ok.
+Proof.
+  split.
+  {
+    simpl.
+     repeat match goal with
+             |[|- is_pf_of_wf_lang (_::_) (?el ++_)] =>
+             let x := open_constr:(_::_) in unify el x; simpl; constructor
+            end.
+     match goal with
+       [|- is_pf_of_wf_lang _ (?g ++ vsubst_elab)]=> unify g (@nil (string * rule_pf)%type); apply is_pf_of_wf_lang_vsubst
+     end.
+     all: try solve [repeat constructor; repeat first [pcon | pvar | by compute]].
+  }
+  {
+    apply /check_lang_okP; by compute.
+  }
+Qed.
+
+(*an extension to subst_eval_ctx++stlc*)
+Definition Estlc :=  
+  [::
+     [:> "G" : #"env",
+       "A" : #"ty",
+       "B" : #"ty",
+       "C" : #"ty",
+       "E" : #"Ectx" %"G" %"C" %"A",
+       "v" : #"val" %"G" (#"->" %"A" %"B"),
+       "e" : #"el" %"G" %"C"
+       ----------------------------------------------- ("plug app_r")
+       #"plug" (#"Eapp_r" %"v" %"E") %"e"
+       = #"app" (#"ret" %"v") (#"plug" %"E" %"e")
+      : #"el" %"G" %"B"
+  ];
+     [:| "G" : #"env",
+       "A" : #"ty",
+       "B" : #"ty",
+       "C" : #"ty",
+       "v" : #"val" %"G" (#"->" %"A" %"B"),
+       "E" : #"Ectx" %"G" %"C" %"A"
+       -----------------------------------------------
+       #"Eapp_r" "v" "E" : #"Ectx" %"G" %"C" %"B"
+  ];
+     [:> "G" : #"env",
+       "A" : #"ty",
+       "B" : #"ty",
+       "C" : #"ty",
+       "E" : #"Ectx" %"G" %"C" (#"->" %"A" %"B"),
+       "e'" : #"el" %"G" %"A",
+       "e" : #"el" %"G" %"C"
+       ----------------------------------------------- ("plug app_l")
+       #"plug" (#"Eapp_l" %"E" %"e'") %"e"
+       = #"app" (#"plug" %"E" %"e") %"e'"
+      : #"el" %"G" %"B"
+  ];
+     [:| "G" : #"env",
+       "A" : #"ty",
+       "B" : #"ty",
+       "C" : #"ty",
+       "E" : #"Ectx" %"G" %"C" (#"->" %"A" %"B"),
+       "e'" : #"el" %"G" %"A"
+       -----------------------------------------------
+       #"Eapp_l" "E" "e'" : #"Ectx" %"G" %"C" %"B"
+  ]]%arule.
+
+
+(*Should be proven using above and embedding properties*)
+Lemma tmp : is_pf_of_wf_lang (subst_eval_ctx ++ stlc) (subst_eval_ctx_elab ++ vstlc_elab).
+Admitted.
+
+Derive Estlc_elab
+       SuchThat (is_pf_of_wf_lang (Estlc ++ subst_eval_ctx ++ stlc) (Estlc_elab ++ subst_eval_ctx_elab ++ vstlc_elab)
+         /\ lang_ok (Estlc_elab ++ subst_eval_ctx_elab ++ vstlc_elab))
+       As Estlc_elab_ok.
+Proof.
+  Arguments subst_eval_ctx : simpl never.
+  Arguments subst_eval_ctx_elab : simpl never.
+  split.
+  {
+    cbn -[subst_eval_ctx subst_eval_ctx_elab stlc vstlc_elab].
+    repeat match goal with
+           |[|-is_pf_of_wf_lang (subst_eval_ctx ++ stlc) (?g ++ subst_eval_ctx_elab ++ vstlc_elab)]=>
+            unify g (@nil (string * rule_pf)%type);  cbn -[subst_eval_ctx subst_eval_ctx_elab stlc vstlc_elab]; apply tmp
+           |[|- is_pf_of_wf_lang (_::_) (?el ++_)] =>
+             let x := open_constr:(_::_) in unify el x;  cbn -[subst_eval_ctx subst_eval_ctx_elab stlc vstlc_elab]; constructor
+           end.
+    
+    all: try solve [repeat constructor; simpl; repeat first [pcon | pvar | by compute]].
+  }
+  {
+    apply /check_lang_okP; by compute.
+  }
+Qed.
+
